Examples/rigidbody1.bpl
@@ -1,4 +1,11 @@
-procedure rigidbody1(x1 : real, x2 : real, x3 : real) returns (r : real) {
-  assume (-15.0 <= x1 && x1 <= 15.0 && -15.0 <= x2 && x2 <= 15.0 && -15.0 <= x3 && x3 <= 15.0);
+procedure rigidbody1(x1 : real, x2 : real, x3 : real) 
+ returns (f : real)
+requires -15e0 <= x1 && x1 <= 15e0;
+requires -15e0 <= x2 && x2 <= 15e0;
+requires -15e0 <= x3 && x3 <= 15e0;
+
+ {
+
   f := -x1*x2 - 2.0 * x2 * x3 - x1 - x3;
 }
+
