Matlab/boundfperror.m
@@ -1,4 +1,9 @@
-function [mf, Mf, mr, Mr, l, h] = boundfperror (p, x, eps, S, B, f, r, relaxOrder, SDPsolverEpsilon)
+function [mf, Mf, mr, Mr, l, h] = boundfperror (delta, x, eps, f, fhat)
+
+S = [1 - x.^2 >= 0]; B = [1 - eps.^2>=0];
+r = f - fhat;
+relaxOrder = 2;
+SDPsolverEpsilon = 1e-9;
 
 sdpsolver = 'sedumi';
 sol = optimize(S, f, sdpsettings('sos.congruence',2, 'solver','sparsepop','sparsepop.relaxOrder',3,'sparsepop.SDPsolver',sdpsolver,'sparsepop.mex',1,'sparsepop.sparseSW',1,'sparsepop.scalingSW',1,'sparsepop.boundSW',2, 'sparsepop.SDPsolverSW',1,'savesolveroutput',1, 'sparsepop.SDPsolverEpsilon',SDPsolverEpsilon));
@@ -7,14 +12,17 @@ sol = optimize(S, -f, sdpsettings('sos.congruence',2, 'solver','sparsepop','spar
 Mf = - sol.solveroutput.SDPobjValue;
 
 mr = 0; Mr = 0;
-delta = 2^(-p);
+tic
 [ralpha monsalpha] = coefficients(r, [x]);
+toc
 nmons = length(ralpha);
 l = 0; h = 0;
+tic
 for alpha = 1:nmons
   [lalpha, halpha] = lhdecompose (ralpha(alpha), [eps]);
   l = l + lalpha*monsalpha(alpha); h = h + halpha*monsalpha(alpha);
 end
+toc
 sol = optimize([S; B], l, sdpsettings('solver','sparsepop','sparsepop.relaxOrder',relaxOrder,'sparsepop.SDPsolver',sdpsolver,'sparsepop.mex',1,'sparsepop.sparseSW',1,'sparsepop.scalingSW',1,'sparsepop.boundSW',2, 'sparsepop.SDPsolverSW',1,'savesolveroutput',1,'sparsepop.SDPsolverEpsilon',SDPsolverEpsilon,'sparsepop.reduceMomentMatSW',1,'sparsepop.multiCliquesFactor',1));
 mr = delta * sol.solveroutput.SDPobjValue;
 sol = optimize([S; B], -l, sdpsettings('sos.congruence',2,'solver','sparsepop','sparsepop.relaxOrder',relaxOrder,'sparsepop.SDPsolver',sdpsolver,'sparsepop.mex',1,'sparsepop.sparseSW',1,'sparsepop.scalingSW',1,'sparsepop.boundSW',2, 'sparsepop.SDPsolverSW',1,'savesolveroutput',1,'sparsepop.SDPsolverEpsilon',SDPsolverEpsilon));
