Matlab/rigidbody1.m
@@ -1,15 +1,15 @@
 clear all;
 close all;
 
-p = 53;
-n = 3; m = 6;
-xscale = sdpvar(n,1);
-eps = sdpvar(m,1);
-x1 = 15 * xscale(1); x2 = 15 * xscale(2); x3 = 15 * xscale(3);
+delta = 2^(-53);
+sdpvar eps0 eps1 eps2 eps3 eps4 eps5;
+sdpvar xscale1 xscale2 xscale3;
+xscale = [xscale1; xscale2; xscale3];
+eps = [eps0; eps1; eps2; eps3; eps4; eps5];
+
+x1 = 15 * xscale1; x2 = 15 * xscale2; x3 = 15 * xscale3;
+
 f = -x1*x2 - 2 * x2 * x3 - x1 - x3;
-fhat = (((-x1 * x2 * (1e0 + eps(1)) - 2 * x2 * (1e0 + eps(2)) * x3 * (1e0 + eps(4))) * (1e0 + eps(5)) - x1) * (1e0 + eps(3)) - x3) * (1e0 + eps(6));
-r = f - fhat;
-S = [1 - xscale(1)^2 >= 0; 1 - xscale(2)^2 >= 0; 1 - xscale(3)^2 >= 0];
-B = [1 - eps(1)^2 >= 0; 1 - eps(2)^2 >= 0; 1 - eps(3)^2 >= 0; 1 - eps(4)^2 >= 0; 1 - eps(5)^2 >= 0; 1 - eps(6)^2 >= 0];
-B = [1 - eps.^2>=0];
-[mf, Mf, mr, Mr] = boundfperror (p, xscale, eps, S, B, f, r, 2, 1e-9);
+f_float = (((-x1 * x2 * (1e0 + eps0) - 2 * x2 * (1e0 + eps1) * x3 * (1e0 + eps3)) * (1e0 + eps4) - x1) * (1e0 + eps2) - x3) * (1e0 + eps5);
+
+[mf, Mf, mr, Mr] = boundfperror (delta, xscale, eps, f, f_float);
